src/3d/prelude/EverParse3d.Actions.fst
@@ -1,0 +1,221 @@
+module EverParse3d.Actions
+friend Prelude
+
+module LPE = LowParse.Low.ErrorCode
+
+let action
+  p inv l on_success a
+=
+    sl: Ghost.erased input_buffer_t ->
+    Stack a
+      (requires fun h ->
+        I.live sl h /\
+        inv sl h /\
+        loc_not_unused_in h `loc_includes` l /\
+        address_liveness_insensitive_locs `loc_includes` l /\
+        l `loc_disjoint` I.footprint sl
+      )
+      (ensures fun h0 _ h1 ->
+        modifies l h0 h1 /\
+        h1 `extends` h0 /\
+        inv sl h1)
+
+module LP = LowParse.Spec.Base
+module LPL = LowParse.Low.Base
+
+unfold
+let valid_pos
+  (#k: LP.parser_kind)
+  (#t: Type)
+  (p: LP.parser k t)
+  (h: HS.mem)
+  (sl: input_buffer_t)
+  (pos: nat)
+  (pos': nat)
+: Tot prop
+= I.live sl h /\
+  begin
+    let s = I.get_remaining sl h in
+    pos <= Seq.length s /\
+    begin match LP.parse p (Seq.slice s pos (Seq.length s)) with
+    | None -> False
+    | Some (_, len) -> pos' == pos + len
+    end
+  end
+
+let valid
+  (#k: LP.parser_kind)
+  (#t: Type)
+  (p: LP.parser k t)
+  (h: HS.mem)
+  (sl: input_buffer_t)
+: Tot prop
+= I.live sl h /\
+  Some? (LP.parse p (I.get_remaining sl h))
+
+let validate_with_action_t' (#k:LP.parser_kind) (#t:Type) (p:LP.parser k t) (inv:slice_inv) (l:eloc) (allow_reading:bool) =
+  (sl: input_buffer_t) ->
+  (startPosition: U64.t) ->
+  Stack U64.t
+  (requires fun h ->
+    I.live sl h /\
+    inv sl h /\
+    loc_not_unused_in h `loc_includes` l /\
+    address_liveness_insensitive_locs `loc_includes` l /\
+    l `loc_disjoint` I.footprint sl /\
+    (allow_reading ==> U64.v startPosition <= Seq.length (I.get_remaining sl h))
+  )
+  (ensures fun h res h' ->
+    I.live sl h' /\
+    modifies (l `loc_union` I.footprint sl) h h' /\
+    h' `extends` h /\
+    inv sl h' /\
+    begin if LPE.is_success res
+    then
+      let pos = if allow_reading then U64.v startPosition else 0 in
+      let s = I.get_remaining sl h in
+      valid_pos p h sl (U64.v res) /\
+      I.get_remaining sl h' == (if allow_reading then s else Seq.slice s (U64.v res) (Seq.length s))
+    else
+      True
+    end
+    )
+
+let validate_with_action_t p inv l allow_reading = validate_with_action_t' p inv l allow_reading
+
+let validate_eta v =
+  fun sl -> v sl
+
+let act_with_comment
+  s res a
+=
+  fun sl ->
+  LPL.comment s;
+  a sl
+
+inline_for_extraction
+let leaf_reader
+  #nz
+  #k
+  (#t: Type)
+  (p: parser k t)
+: Tot Type
+= (sl: input_buffer_t) ->
+  Stack t
+  (requires (fun h ->
+    valid p h sl
+  ))
+  (ensures (fun h res h' ->
+    let s = I.get_remaining sl h in
+    I.live sl h' /\
+    modifies (I.footprint sl) h h' /\
+    h' `extends` h /\
+    begin match LP.parse p s with
+    | None -> False
+    | Some (y, len) ->
+      res == y /\
+      I.get_remaining sl h' == Seq.slice s len (Seq.length s)
+    end
+  ))
+
+
+inline_for_extraction
+noextract
+let validate_with_success_action' (name: string) #nz #wk (#k1:parser_kind nz wk) #t1 (#p1:parser k1 t1) (#inv1:_) (#l1:eloc) (#ar:_)
+                         (v1:validate_with_action_t p1 inv1 l1 ar)
+                         (#inv2:_) (#l2:eloc) #b (a:action p1 inv2 l2 b bool)
+  : validate_with_action_t p1 (conj_inv inv1 inv2) (l1 `eloc_union` l2) ar
+  = fun input startPosition ->
+    let h0 = HST.get () in
+    [@(rename_let ("positionAfter" ^ name))]
+    let pos1 = v1 input startPosition in
+    let h1 = HST.get () in
+    modifies_address_liveness_insensitive_unused_in h0 h1;
+    if LPL.is_success pos1
+    then
+         [@(rename_let ("action_success_" ^ name))]
+         let b = a input in
+         if not b
+         then validator_error_action_failed
+         else pos1
+    else
+         pos1
+
+inline_for_extraction
+noextract
+let validate_drop_true
+   #nz #wk (#k:parser_kind nz wk) (#t:Type) (#p:parser k t) (#inv:slice_inv) (#l:eloc) (v: validate_with_action_t p inv l true)
+: Tot (validate_with_action_t p inv l false)
+= fun input startPosition ->
+  let res = v input startPosition in
+  if LPE.is_success res
+  then begin
+    let h1 = HST.get () in
+    I.skip input (LPE.uint64_to_uint32 (res `U64.sub` startPosition));
+    let h2 = HST.get () in
+    assert (h2 `extends` h1)
+  end;
+  res
+
+inline_for_extraction
+noextract
+let validate_drop
+   #nz #wk (#k:parser_kind nz wk) (#t:Type) (#p:parser k t) (#inv:slice_inv) (#l:eloc) #allow_reading (v: validate_with_action_t p inv l allow_reading)
+: Tot (validate_with_action_t p inv l false)
+= if allow_reading
+  then validate_drop_true v
+  else v
+
+let validate_with_success_action
+  name v1 a
+= validate_drop (validate_with_success_action' name v1 a)
+
+inline_for_extraction noextract
+let validate_with_error_action' (name: string) #nz #wk (#k1:parser_kind nz wk) #t1 (#p1:parser k1 t1) (#inv1:_) (#l1:eloc) (#ar:_)
+                         (v1:validate_with_action_t p1 inv1 l1 ar)
+                         (#inv2:_) (#l2:eloc) (a:action p1 inv2 l2 false bool)
+  : validate_with_action_t p1 (conj_inv inv1 inv2) (l1 `eloc_union` l2) ar
+  = fun input startPosition ->
+    let h0 = HST.get () in
+    [@(rename_let ("positionAfter" ^ name))]
+    let pos1 = v1 input startPosition in
+    let h1 = HST.get () in
+    modifies_address_liveness_insensitive_unused_in h0 h1;
+    if LPL.is_success pos1
+    then pos1
+    else
+         [@(rename_let ("action_error_" ^ name))]
+         let b = a input in
+         if not b then validator_error_action_failed else pos1
+
+let validate_with_error_action
+  name v1 a
+= validate_drop (validate_with_error_action' name v1 a)
+
+inline_for_extraction noextract
+let validate_ret
+  : validate_with_action_t (parse_ret ()) true_inv eloc_none true
+  = fun input startPosition ->
+    startPosition
+
+#push-options "--z3rlimit 16"
+
+inline_for_extraction noextract
+let validate_pair'
+       (name1: string)
+       #nz1 (#k1:parser_kind nz1 WeakKindStrongPrefix) #t1 (#p1:parser k1 t1)
+       (#inv1:_) (#l1:eloc) (#ar1:_) (v1:validate_with_action_t p1 inv1 l1 ar1)
+       #nz2 #wk2 (#k2:parser_kind nz2 wk2) #t2 (#p2:parser k2 t2)
+       (#inv2:_) (#l2:eloc) (#ar2:_) (v2:validate_with_action_t p2 inv2 l2 ar2)
+  : validate_with_action_t (p1 `parse_pair` p2) (conj_inv inv1 inv2) (l1 `eloc_union` l2) (ar1 && ar2)
+  = fun input startPosition ->
+    let h = HST.get () in
+    [@(rename_let ("positionAfter" ^ name1))]
+    let pos1 = v1 input startPosition in
+    let h1 = HST.get () in
+    modifies_address_liveness_insensitive_unused_in h h1;
+    if LPL.is_error pos1
+    then
+      pos1
+    else
+      v2 input pos1
